further test

tests/lean/run/cbv1.lean
@@ -5,11 +5,96 @@ def myId (n : myNat) : myNat := n
 def natFun (n : Nat) : Nat := match n with
   | 0 => 0
   | n + 1 => (natFun n).succ
-  termination_by n
 
-theorem myTest0 : (fun x y => y) (myId 1) (myId 2) = 2:= by
+
+def test (b : Bool) : Bool := match b,(!b) with
+| true, true => false
+| false, true => false
+| true, false => false
+| false, false => true
+
+#check test.match_1.congr_eq_4
+
+theorem myTest0 : 2 * 2 = 4 := by
   conv =>
     lhs
     cbv
 
-#print myTest0
+def ident := String deriving BEq, Repr, Hashable
+
+/-
+  The abstract syntax: an arithmetic expression is either...
+-/
+inductive aexp : Type where
+  | CONST (n : Int)               -- a constant, or
+  | VAR (x : ident)               -- a variable, or
+  | PLUS (a1 : aexp) (a2 : aexp)  -- a sum of two expressions, or
+  | MINUS (a1 : aexp) (s2 : aexp) -- a difference of two expressions
+
+/-
+  The denotational semantics: an evaluation function that computes the integer value denoted by an expression.  It is parameterized by a store [s] that associates values to variables.
+-/
+
+def store : Type := ident → Int
+
+@[grind] def aeval (s : store) (a : aexp) : Int :=
+  match a with
+  | .CONST n => n
+  | .VAR x => s x
+  | .PLUS a1 a2 => aeval s a1 + aeval s a2
+  | .MINUS a1 a2 => aeval s a1 - aeval s a2
+
+inductive bexp : Type where
+  | TRUE                              -- always true
+  | FALSE                             -- always false
+  | EQUAL (a1 : aexp) (a2 : aexp)     -- whether [a1=a]
+  | LESSEQUAL (a1 : aexp) (a2 : aexp) -- whether [a1≤a]
+  | NOT (b1 : bexp)                   -- Boolean negation
+  | AND (b1 : bexp) (b2 : bexp)       -- Boolean conjunction
+
+@[grind] def beval (s : store) (b : bexp) : Bool :=
+  match b with
+  | .TRUE => true
+  | .FALSE => false
+  | .EQUAL a1 a2 => aeval s a1 = aeval s a2
+  | .LESSEQUAL a1 a2 => aeval s a1 <= aeval s a2
+  | .NOT b1 =>  !(beval s b1)
+  | .AND b1 b2 => beval s b1 && beval s b2
+
+inductive com : Type where
+  | SKIP                                        -- do nothing
+  | ASSIGN (x : ident) (a : aexp)               -- assignment: [v := a]
+  | SEQ (c1 : com) (c2 : com)                   -- sequence: [c1; c2]
+  | IFTHENELSE (b : bexp) (c1 : com) (c2 : com) -- conditional: [if b then c1 else c2]
+  | WHILE (b : bexp) (c1 : com)                 -- loop: [while b do c1 done]
+
+@[grind] def update (x : ident) (v : Int) (s : store) : store :=
+  fun y => if x == y then v else s y
+
+@[grind] def cexec_bounded (fuel : Nat) (s : store) (c : com) : Option store :=
+  match fuel with
+  | .zero => .none
+  | .succ fuel' =>
+    match c with
+    | .SKIP => .some s
+    | .ASSIGN x a => .some (update x (aeval s a) s)
+    | .SEQ c1 c2 =>
+      match cexec_bounded fuel' s c1 with
+      | .none => .none
+      | .some s' => cexec_bounded fuel' s' c2
+    | .IFTHENELSE b c1 c2 =>
+      if beval s b then cexec_bounded fuel' s c1 else cexec_bounded fuel' s c2
+    | .WHILE b c1 =>
+      if beval s b then
+        match cexec_bounded fuel' s c1 with
+        | .none => .none
+        | .some s' => cexec_bounded fuel' s' (.WHILE b c1)
+      else
+        .some s
+
+/- Violates an assertion -/
+theorem cexec1 : cexec_bounded 1 (fun _ => 0) (.SKIP) = sorry := by
+  conv =>
+    lhs
+    cbv
+  sorry
